More inst2 cleanup.

attic/Apply_Trace_Cmd.thy
@@ -60,6 +60,22 @@ begin
    apply_trace (rule X)
    oops
 end
+experiment begin
+text \<open>Example of trace for grouped lemmas\<close>
+definition ex :: "nat set"  where
+ "ex = {1,2,3,4}"
 
+lemma v1:  "1 \<in> ex"  by (simp add: ex_def)
+lemma v2:  "2 \<in> ex"  by (simp add: ex_def)
+lemma v3:  "3 \<in> ex"  by (simp add: ex_def)
 
+text \<open>Group several lemmas in a single one\<close>
+lemmas vs = v1 v2 v3
+
+lemma "2 \<in> ex"
+  apply_trace \<open>"_\<in>_"\<close> (simp add: vs vs)
+    find_theorems (with_dups) "2 \<in> ex"
+  oops
+
+end
 end
